steel/Zeta.Steel.IArray.fsti
@@ -15,8 +15,19 @@ val tbl (#k:eqtype)
         (vp:EHT.vp_t k v contents)
   : Type0
 
-let repr (k:eqtype) (contents:Type0) = m:Map.t k contents { Map.domain m `Set.equal` Set.complement Set.empty }
+let repr (k:eqtype)
+         (contents:Type0)
+  : Type0
+  = m:Map.t k contents { Map.domain m `Set.equal` Set.complement Set.empty }
 
+let borrows (k:eqtype)
+            (v:Type0)
+  : Type0
+  = FStar.PartialMap.t k v
+
+let empty_borrows #k #v 
+  : borrows k v
+  = PartialMap.empty k v
 
 (* perm t m b: asserts ownership of the underlying array
 
@@ -35,31 +46,77 @@ val perm (#k:eqtype)
          (#vp:EHT.vp_t k v contents)
          (t:tbl h vp)
          ([@@@smt_fallback] m:repr k contents)
+         ([@@@smt_fallback] b:borrows k v)
   : vprop
 
+[@@__steel_reduce__; __reduce__]
+let full_perm (#k:eqtype)
+              (#v:Type0)
+              (#contents:Type0)
+              (#h:EHT.hash_fn k)
+              (#vp:EHT.vp_t k v contents)
+              (t:tbl h vp)
+              ([@@@smt_fallback] m:repr k contents)
+  = perm t m empty_borrows
+         
 val create (#k:eqtype)
            (#v:Type0)
            (#contents:Type0)
            (#vp:EHT.vp_t k v contents)
            (h:EHT.hash_fn k)
            (n:U32.t{U32.v n > 0})
-           (finalize:EHT.finalizer_t vp)
            (init:Ghost.erased contents)
-  : STT (tbl h vp) emp (fun a -> perm a (Map.const #k #contents init))
+  : STT (tbl h vp) emp (fun a -> perm a (Map.const #k #contents init) empty_borrows)
 
-
-(* Call the finalizer on every value stored in memory
-   and then frees the array itself *)
+(* Call the finalizer on the array only.
+   Freeing every element of the array is up to the client *)
 val free (#k:eqtype)
          (#v:Type0)
          (#h:EHT.hash_fn k)
          (#contents: Type0)
          (#vp:EHT.vp_t k v contents)
          (#m:G.erased (repr k contents))
+         (#b:G.erased (borrows k v))
          (a:tbl h vp)
   : STT unit
-      (perm a m)
+      (perm a m b)
       (fun _ -> emp)
+
+
+let get_post 
+  (#k:eqtype)
+  (#v #contents:Type0)
+  (#vp:EHT.vp_t k v contents)
+  (#h:EHT.hash_fn k)
+  (m:G.erased (repr k contents))
+  (borrows:G.erased (borrows k v))
+  (a:tbl h vp)
+  (i:k)
+  : EHT.get_result k v -> vprop
+  = fun r ->
+    match r with
+    | EHT.Present x ->
+      perm a m (PartialMap.upd i x borrows)  //when `get` succeeds, the key is added to `borrows`
+        `star`
+      vp i x (Map.sel m i)                   //in addition, we return the vp permission for the key
+
+    | _ ->
+      perm a m borrows
+
+val get
+  (#k:eqtype)
+  (#v #contents:Type0)
+  (#vp:EHT.vp_t k v contents)
+  (#h:EHT.hash_fn k)
+  (#m:G.erased (repr k contents))
+  (#borrows:G.erased (borrows k v))
+  (a:tbl h vp)
+  (i:k)
+  : ST (EHT.get_result k v)
+       (perm a m borrows)
+       (get_post m borrows a i)
+       (requires ~ (PartialMap.contains i borrows))
+       (ensures fun _ -> True)
 
 (* If i happens to collide with an existing key i' in memory
    then then i' is vacated and the finalizer is called on its contents *)
@@ -69,26 +126,36 @@ val put (#k:eqtype)
         (#h:EHT.hash_fn k)
         (#vp:EHT.vp_t k v contents)
         (#m:G.erased (repr k contents))
+        (#b:G.erased (borrows k v))
         (a:tbl h vp)
         (i:k)
         (x:v)
         (c:Ghost.erased contents)
   : STT unit
-      (perm a m `star` vp i x c)
-      (fun _ -> perm a (Map.upd m i c))
+      (perm a m b `star` vp i x c)
+      (fun _ -> perm a (Map.upd m i c) (PartialMap.remove i b))
 
-val remove
-  (#k:eqtype)
-  (#v #contents:Type0)
-  (#h:EHT.hash_fn k)
-  (#vp:EHT.vp_t k v contents)
-  (#m:G.erased (repr k contents))
-  (a:tbl h vp)
-  (i:k)
-  : STT bool
-        (perm a m)
-        (fun _ -> perm a m)
 
+val ghost_put
+        (#o:_)
+        (#k:eqtype)
+        (#v:Type0)
+        (#contents:Type0)
+        (#h:EHT.hash_fn k)
+        (#vp:EHT.vp_t k v contents)
+        (#m:G.erased (repr k contents))
+        (#b:G.erased (borrows k v))
+        (a:tbl h vp)
+        (i:k)
+        (x:v)
+        (c:Ghost.erased contents)
+  : STGhost unit o
+      (perm a m b `star` vp i x c)
+      (fun _ -> perm a (Map.upd m i c) (PartialMap.remove i b))
+      (requires
+        PartialMap.sel i b == Some x)
+      (ensures fun _ -> 
+        True)
 
 let with_key_post_present_predicate
   (#k:eqtype)
@@ -96,6 +163,7 @@ let with_key_post_present_predicate
   (#vp:EHT.vp_t k v contents)
   (#h:EHT.hash_fn k)
   (m:G.erased (repr k contents))
+  (b:G.erased (borrows k v))
   (a:tbl h vp)
   (i:k)
   (#res:Type)
@@ -103,7 +171,7 @@ let with_key_post_present_predicate
   (r:res)
   : contents -> vprop
   = fun c' ->
-    perm a (Map.upd m i c')
+    perm a (Map.upd m i c') b
       `star`
     f_post (Map.sel m i) c' r
   
@@ -113,6 +181,7 @@ let with_key_post
   (#vp:EHT.vp_t k v contents)
   (#h:EHT.hash_fn k)
   (m:G.erased (repr k contents))
+  (b:G.erased (borrows k v))
   (a:tbl h vp)
   (i:k)
   (#res:Type)
@@ -122,9 +191,9 @@ let with_key_post
   = fun r ->
     match r with
     | EHT.Present res ->
-      exists_ (with_key_post_present_predicate m a i f_post res)
+      exists_ (with_key_post_present_predicate m b a i f_post res)
     | _ ->
-      perm a m
+      perm a m b
         `star`
       f_pre
 
@@ -134,6 +203,7 @@ val with_key
   (#vp:EHT.vp_t k v contents)
   (#h:EHT.hash_fn k)
   (#m:G.erased (repr k contents))
+  (#b:G.erased (borrows k v))  
   (a:tbl h vp)
   (i:k)
   (#res:Type)
@@ -142,9 +212,11 @@ val with_key
   ($f:(x:v -> STT res
              (f_pre `star` vp i x (Map.sel m i))
              (fun res -> exists_ (fun c' -> f_post (Map.sel m i) c' res `star` vp i x c'))))
-  : STT (EHT.get_result k res)
-        (perm a m `star` f_pre)
-        (with_key_post m a i f_pre f_post)
+  : ST (EHT.get_result k res)
+       (perm a m b `star` f_pre)
+       (with_key_post m b a i f_pre f_post)
+       (requires ~(PartialMap.contains i b))
+       (ensures fun _ -> True)
 
 let elim_with_key_post_present
         #o
@@ -153,6 +225,7 @@ let elim_with_key_post_present
         (#vp:EHT.vp_t k v contents)
         (#h:EHT.hash_fn k)
         (#m:G.erased (repr k contents))
+        (#b:G.erased (borrows k v))        
         (#a:tbl h vp)
         (#i:k)
         (#res:Type)
@@ -160,14 +233,14 @@ let elim_with_key_post_present
         (#f_post:contents -> contents -> res -> vprop)
         (r:res)
   : STGhostT (G.erased contents) o
-    (with_key_post m a i f_pre f_post (EHT.Present r))
+    (with_key_post m b a i f_pre f_post (EHT.Present r))
     (fun c' ->
-       perm a (Map.upd m i c')
+       perm a (Map.upd m i c') b
          `star`
        f_post (Map.sel m i) c' r)
   = rewrite
-      (with_key_post m a i f_pre f_post (EHT.Present r))
-      (exists_ (with_key_post_present_predicate m a i f_post r));
+      (with_key_post m b a i f_pre f_post (EHT.Present r))
+      (exists_ (with_key_post_present_predicate m b a i f_post r));
     let c' = elim_exists () in
-    rewrite (with_key_post_present_predicate m a i f_post r c') _;
+    rewrite (with_key_post_present_predicate m b a i f_post r c') _;
     c'
